{
 "cells": [
  {
   "cell_type": "markdown",
   "metadata": {},
   "source": [
    "## Тема 8 “Понятие об интеграле”"
   ]
  },
  {
   "cell_type": "markdown",
   "metadata": {},
   "source": [
    "   ### 8.1. Найти неопределенный интеграл:\n",
    "  $\\int_{}^{}(2x^2 - 2x - 1 + sin(x) - cos(x) + ln{x} + e^x)dx$"
   ]
  },
  {
   "cell_type": "markdown",
   "metadata": {},
   "source": [
    " $\\int_{}^{}(2x^2 - 2x - 1 + sin(x) - cos(x) + ln{x} + e^x)dx$ = <br> = $\\int_{}^{}(2x^2)dx$ -  $\\int_{}^{}(2x)dx$ -  $\\int_{}^{}(1)dx$ +  $\\int_{}^{}(sin{x})dx$ - $\\int_{}^{}(cos{x})dx$ +  $\\int_{}^{}(ln{x})dx$ +  $\\int_{}^{}(e^x)dx$ = <br>  = $2\\frac{x^3}{3} - x^2 - x -\\cos{x} - \\sin{x} + x\\ln{x} - x + e^x + C$ = <br> = $2\\frac{x^3}{3} - x^2 - 2x -\\cos{x} - \\sin{x} + x\\ln{x} + e^x + C$"
   ]
  },
  {
   "cell_type": "markdown",
   "metadata": {},
   "source": [
    "   ### 8.2. Найти неопределенный интеграл:\n",
    "  $\\int_{}^{}(2x + 6xz^2 - 5x^2y - 3ln{z})dx$"
   ]
  },
  {
   "cell_type": "markdown",
   "metadata": {},
   "source": [
    " $\\int_{}^{}(2x + 6xz^2 - 5x^2y - 3ln{z})dx = \\int_{}^{}(2x)dx + \\int_{}^{}(6xz^2)dx - \\int_{}^{}(5x^2y)dx - \\int_{}^{}(3ln{z})dx$ <br> $= x^2 + 6z^2 \\frac{x^2}{2} - 5y \\frac{x^3}{3} - x3ln{z} + C$ $= x^2 + 3z^2 x^2 -  \\frac{5y x^3}{3} - 3xln{z} + C$"
   ]
  },
  {
   "cell_type": "markdown",
   "metadata": {},
   "source": [
    "### 8.3. Вычислить определенный интеграл:\n",
    "$\\int_{0}^{\\pi}3x^2sin(2x)dx$, $\\int_{}^{}udv$ = $uv - \\int_{}^{}vdu$"
   ]
  },
  {
   "cell_type": "markdown",
   "metadata": {},
   "source": [
    "$u = x^2, du = 2xdx$ <br>$dv = 3sin(2x)dx, v = -\\frac{3}{2}cos{2x}$"
   ]
  },
  {
   "cell_type": "markdown",
   "metadata": {},
   "source": [
    "$\\int_{}^{}3x^2sin(2x)dx = x^2(-\\frac{3}{2}cos{2x}) -\\int_{}^{}-\\frac{3}{2}cos{(2x)}*2xdx =$<br> =$ x^2(-\\frac{3}{2}cos{2x}) -\\int_{}^{}-\\frac{3}{2}cos{(2x)}*2xdx$ = $ -\\frac{3}{2}x^2cos{2x} +\\frac{3}{2}\\int_{}^{}2xcos{(2x)}dx = $<br> = $ -\\frac{3}{2}x^2cos{2x} +\\frac{3}{4}\\int_{}^{}2xcos{(2x)}d(2x)  =(1)$"
   ]
  },
  {
   "cell_type": "code",
   "execution_count": null,
   "metadata": {},
   "outputs": [],
   "source": []
  },
  {
   "cell_type": "markdown",
   "metadata": {},
   "source": [
    "$\\int_{}^{}2xcos{(2x)}d(2x), y = 2x $ => $\\int_{}^{}y*cos{(y)}*dy  $"
   ]
  },
  {
   "cell_type": "markdown",
   "metadata": {},
   "source": [
    " $\\int_{}^{}udv$ = $uv - \\int_{}^{}vdu$<br> $ u = y => du=dy  $<br>$dV = \\cos{(y)} => V = sin(y) $"
   ]
  },
  {
   "cell_type": "markdown",
   "metadata": {},
   "source": [
    "$y*\\sin{y} -\\int_{}^{}\\sin{y}dy = y*\\sin{y} + \\cos{y} , y = 2x => 2x\\sin{(2x)} + \\cos{(2x)}$"
   ]
  },
  {
   "cell_type": "code",
   "execution_count": null,
   "metadata": {},
   "outputs": [],
   "source": []
  },
  {
   "cell_type": "markdown",
   "metadata": {},
   "source": [
    "$(1)= -\\frac{3}{2}x^2cos{2x} + \\frac{3}{4}(2x\\sin{(2x)} + \\cos{(2x)}) + C$ "
   ]
  },
  {
   "cell_type": "markdown",
   "metadata": {},
   "source": [
    "$cos(2\\pi) = 1$ ,$cos(0) = 1$ <br>\n",
    "$sin(2\\pi) = 0$, $sin(0) = 0$ <br>"
   ]
  },
  {
   "cell_type": "markdown",
   "metadata": {},
   "source": [
    "$F{(\\pi)}= -\\frac{3}{2}\\pi^2 \\cos{2\\pi} + \\frac{3}{4}(2\\pi\\sin{(2\\pi)} + \\cos{(2\\pi)}) = -\\frac{3}{2}\\pi^2 + \\frac{3}{4}(2\\pi*0 + 1)= -\\frac{3}{2}\\pi^2 + \\frac{3}{4}$"
   ]
  },
  {
   "cell_type": "markdown",
   "metadata": {},
   "source": [
    "$F{(0)}= -\\frac{3}{2}0^2 \\cos{2*0} + \\frac{3}{4}(2*0*sin{(2*0)} + \\cos{(2*0)}) = \\frac{3}{4}\\cos{(0)} = \\frac{3}{4} $"
   ]
  },
  {
   "cell_type": "markdown",
   "metadata": {},
   "source": [
    "$\\int_{0}^{\\pi}3x^2sin(2x)dx =  -\\frac{3}{2}\\pi^2 + \\frac{3}{4} - \\frac{3}{4} = -\\frac{3}{2}\\pi^2 $"
   ]
  },
  {
   "cell_type": "markdown",
   "metadata": {},
   "source": [
    "### 8.4. Найти неопределенный интеграл:\n",
    "$\\int_{}^{}\\frac{1}{\\sqrt{x+1}}dx$"
   ]
  },
  {
   "cell_type": "markdown",
   "metadata": {},
   "source": [
    "### $\\int_{}^{}\\frac{1}{\\sqrt{x+1}}dx = \\int_{}^{}(x+1)^{-\\frac{1}{2}}dx$"
   ]
  },
  {
   "cell_type": "markdown",
   "metadata": {},
   "source": [
    "$ (x+1)=t => x=(t-1) => dx = dt $"
   ]
  },
  {
   "cell_type": "markdown",
   "metadata": {},
   "source": [
    "### $ \\int{}^{}u^ndu = \\frac{u^{n+1}}{n+1} $"
   ]
  },
  {
   "cell_type": "markdown",
   "metadata": {},
   "source": [
    "### $ \\int_{}^{}t^{-\\frac{1}{2}}dt =$ $\\frac{t^\\frac{1}{2}}{\\frac{1}{2}} + C = 2t^\\frac{1}{2} + C => 2(x+1)^\\frac{1}{2} + C = 2\\sqrt{x+1} + C$ "
   ]
  },
  {
   "cell_type": "code",
   "execution_count": null,
   "metadata": {},
   "outputs": [],
   "source": []
  }
 ],
 "metadata": {
  "kernelspec": {
   "display_name": "Python 3",
   "language": "python",
   "name": "python3"
  },
  "language_info": {
   "codemirror_mode": {
    "name": "ipython",
    "version": 3
   },
   "file_extension": ".py",
   "mimetype": "text/x-python",
   "name": "python",
   "nbconvert_exporter": "python",
   "pygments_lexer": "ipython3",
   "version": "3.8.5"
  }
 },
 "nbformat": 4,
 "nbformat_minor": 4
}
